format-version: 1.4
date: 20:05:2011 14:15
saved-by: zhutchok
auto-generated-by: The OWL API (version 3.2.2.1502)
id_space: rdfs http://www.w3.org/2000/01/rdf-schema#
id_space: owl http://www.w3.org/2002/07/owl#
id_space: oboInOwl http://www.geneontology.org/formats/oboInOwl#
id_space: rdf http://www.w3.org/1999/02/22-rdf-syntax-ns#
id_space: KISAO http://www.biomodels.net/kisao/KISAO#
id_space: xsd http://www.w3.org/2001/XMLSchema#
remark: Kinetic Simulation Algorithm Ontology
versionInfo: 2.0


! ----------------------  PROPERTIES  -------------------------

[Typedef]
id: KISAO:0000245
name: has characteristic
namespace: KISAO
domain: KISAO:0000000
range: KISAO:0000097
is_metadata_tag: false

[Typedef]
id: KISAO:0000246
name: is hybrid of
namespace: KISAO
def: "The basic idea of hybrid simulation methods is to combine the advantages of complementary simulation approaches: the whole system is subdivided into appropriate parts and different simulation methods operate on these parts at the same time." [urn:miriam:doi:10.1093/bib/bbn050 "Biochemical simulations: stochastic, approximate stochastic and hybrid approaches. Pahle J. Brief Bioinform. 2009 Jan;10(1):53-64. Epub 2009 Jan 16."]
domain: KISAO:0000000
range: KISAO:0000000
is_metadata_tag: false

[Typedef]
id: KISAO:0000247
name: lacks property
namespace: KISAO
def: "lacksProperty is an alias for not hasProperty. It should not be used in OWL version of KiSAO. It's used in OBO version of KiSAO, as it is not possible to represent negation in OBO." [:]
domain: KISAO:0000000
range: KISAO:0000097
is_metadata_tag: false
owldef: "?X subclassOf not (KISAO:0000245 some ?Y)"

[Typedef]
id: KISAO:0000250
name: is parameter of
namespace: KISAO
def: "Links parameters to the algorithms which use them." [:]
domain: KISAO:0000201
range: KISAO:0000000
inverse: KISAO:0000259
is_metadata_tag: false

[Typedef]
id: KISAO:0000259
name: has parameter
namespace: KISAO
def: "Links algorithms to the parameters they use." [:]
domain: KISAO:0000000
range: KISAO:0000201
inverse: KISAO:0000250
is_metadata_tag: false


! ----------------------  DATA PROPERTIES  -------------------------

[Typedef]
id: KISAO:0000251
name: has type
namespace: KISAO
def: "Indicates the type of algorithm parameter value, such as, for example, xsd:integer." [:]
domain: KISAO:0000201
is_metadata_tag: false


! ----------------------  CLASSES  -------------------------

[Term]
id: KISAO:0000000
name: kinetic simulation algorithm
namespace: KISAO
def: "Algorithm used to instantiate a simulation from a mathematical model, where the variable values evolve over time." [:]
disjoint_from: KISAO:0000097
disjoint_from: KISAO:0000201
creation_date: 2008-05-26T00:00:00Z
created_by: dk

[Term]
id: KISAO:0000001
name: Gillespie-like approximate stochastic simulation method
namespace: KISAO
is_obsolete: true
replaced_by: KISAO:0000025^KISAO:0000245(KISAO:0000237)

[Term]
id: KISAO:0000002
name: non-spatial tau-leaping method
namespace: KISAO
is_obsolete: true

[Term]
id: KISAO:0000003
name: weighted SSA
namespace: KISAO
def: "The weighted Stochastic Simulation Algorithm manipulates the probabilities measure of biochemical systems by sampling, in order to increase the fraction of simulation runs exhibiting rare events." [urn:miriam:pubmed:19045316 "Kuwahara H, Mura I. (2008) An efficient and exact stochastic simulation method to analyze rare events in biochemical systems. J Chem Phys. 129(16):165101."]
is_a: KISAO:0000034
disjoint_from: KISAO:0000038
disjoint_from: KISAO:0000015
disjoint_from: KISAO:0000027
creation_date: 2009-01-24T00:00:00Z
created_by: NLN

[Term]
id: KISAO:0000015
name: Gillespie's first reaction method
namespace: KISAO
def: "Stochastic simulation algorithm using the next-reaction density function, giving the probability that the next reaction will happen in a given time interval. To choose the next reaction to fire, the algorithm calculates a tentative reaction time for each reaction and then select the smallest." [urn:miriam:doi:10.1016/0021-9991(76)90041-3 "Gillespie DT. A General Method for Numerically Simulating the Stochastic Time Evolution of Coupled Chemical Reactions. Journal of Computational Physics, Volume 2 , pages 403-434 (1976)."]
is_a: KISAO:0000034
disjoint_from: KISAO:0000003
disjoint_from: KISAO:0000038
disjoint_from: KISAO:0000027
creation_date: 2007-10-09T00:00:00Z
created_by: NLN

[Term]
id: KISAO:0000016
name: algorithm using discrete variables
namespace: KISAO
def: "Algorithm that allows to change the values of a system's variables by discrete (integral) amounts." [:]
is_obsolete: true
replaced_by: KISAO:0000000^KISAO:0000245(KISAO:0000105)
creation_date: 2008-07-08T00:00:00Z
created_by: NLN

[Term]
id: KISAO:0000017
name: multi-state agent-based simulation method
namespace: KISAO
def: "The agent-based simulation method instantiates each molecule as an individual software object. The interactions between those objects are determined by interaction probabilities according to experimental data. The probability is depended on the state the molecule is in at that specific time (molecules have multiple-state). Additionally, ''pseudo-molecules'' are introduced to the system in order to simulate unimolecular reactions. For simulation, continuous time is broken down into disrete, independent ''slices''. During each time slice one molecule is selected randomly, a second molecule or pseudo-molecule is selected afterwards (leading to either a unimolecular or a bimolecular reaction). The reaction will only take place if a produced random number exceeds the reaction probability calculated beforehand. In that case, the system is updated after that reaction." [urn:miriam:pubmed:9628844 "Morton-Firth, C.J, Bray, D. Predicting temporal fluctuations in an intracellular signalling pathway. Journal of Theoretical Biology, volume 192, pages 117-128 (1998)."]
comment: The agent-based simulation method is, for example, used in StochSim.
synonym: "Morton-Firth" EXACT []
is_a: KISAO:0000000
disjoint_from: KISAO:0000056
disjoint_from: KISAO:0000264
disjoint_from: KISAO:0000094
disjoint_from: KISAO:0000241
disjoint_from: KISAO:0000261
disjoint_from: KISAO:0000064
disjoint_from: KISAO:0000019
disjoint_from: KISAO:0000231
relationship: KISAO:0000245 KISAO:0000108

relationship: KISAO:0000247 KISAO:0000102

relationship: KISAO:0000245 KISAO:0000104

relationship: KISAO:0000245 KISAO:0000105


[Term]
id: KISAO:0000018
name: algorithm using continuous variables
namespace: KISAO
def: "Algorithm that allows to change the values of a system's variables by continuous (non-integral) amounts." [:]
is_obsolete: true
replaced_by: KISAO:0000000^KISAO:0000245(KISAO:0000106)
creation_date: 2008-07-08T00:00:00Z
created_by: NLN

[Term]
id: KISAO:0000019
name: CVODE
namespace: KISAO
def: "The CVODE is a package written in C that solves initial value problems for ODEs. It is capable for stiff and non-stiff systems and uses two different linear multi-step methods, namely the Adam-Moulton method and the Backward differentiation formula (BNF)." [citeulike:1832863 "Cohen S, Hindmarsh C. Cvode, A Stiff/nonstiff Ode Solver In C. Computers in Physics, Vol. 10 (2), pages 138-143 (1996)."]
synonym: "code value ordinary differential equation solver" EXACT []
is_a: KISAO:0000000
disjoint_from: KISAO:0000056
disjoint_from: KISAO:0000264
disjoint_from: KISAO:0000094
disjoint_from: KISAO:0000241
disjoint_from: KISAO:0000261
disjoint_from: KISAO:0000064
disjoint_from: KISAO:0000017
disjoint_from: KISAO:0000231
relationship: KISAO:0000245 KISAO:0000103

relationship: KISAO:0000247 KISAO:0000102

relationship: KISAO:0000245 KISAO:0000107

relationship: KISAO:0000245 KISAO:0000106

creation_date: 2007-10-30T00:00:00Z
created_by: dk

[Term]
id: KISAO:0000020
name: PVODE
namespace: KISAO
def: "PVODE is a general-purpose solver for ordinary differential equation (ODE) systems that implements methods for both stiff and nonstiff systems. [...] In the stiff case, PVODE uses a backward differentiation formula method combined with preconditioned GMRES iteration. Parallelism is achieved by distributing the ODE solution vector into user-specified segments and parallelizing a set of vector kernels accordingly. For PDE-based ODE systems, we provide a module that generates a band block-diagonal preconditioner for use with the GMRES iteration. " [urn:miriam:doi:10.1177/109434209901300405 "Byrne GD, Hindmarsh AC. PVODE, an ODE Solver for Parallel Computers. International Journal of High Performance Computing Applications, Vol. 13 (4), pages 354-365 (1999)."]
synonym: "parallel code value ordinary differential equation solver" EXACT []
is_a: KISAO:0000019

[Term]
id: KISAO:0000021
name: StochSim nearest-neighbour algorithm
namespace: KISAO
def: "The nearest-neighbor algorithm allows for the representation of spatial information, by adding a two-dimensional lattice in the form of a probabilistic cellular automata. That way, nearest neighbor interactions do additionally influence reactions taking place in the systems. Reactions between entities are calculated using the agent-based simulation algorithm." [urn:miriam:pubmed:11395441 "Le Novere N, Shimizu TS. STOCHSIM: modelling of stochastic biomolecular processes. Bioinformatics, volume 17 (6), pages 575-576 (2001)."]
comment: The nearest-neighbor algorithm is for example used in Stochsim 1.2 and more recent versions.
is_a: KISAO:0000264
disjoint_from: KISAO:0000068
relationship: KISAO:0000245 KISAO:0000104


[Term]
id: KISAO:0000022
name: next-subvolume method
namespace: KISAO
def: "Sub-volume stochastic reaction-diffusion method that is a combination of the Direct Method [KISAO:0000029] for sampling the time for a next reaction or diffusion event in each subvolume, with Gibson and Bruck's Next Reaction Method [NRM, KISAO:0000027], which is used to keep track of in which subvolume an event occurs next. The subvolumes are kept sorted in a queue, implemented as a binary tree, according to increasing time of the next event. When an event has occurred in the subvolume at the top of the queue, new event times need to be sampled only for one (the event is a chemical reaction) or two (the event is a diffusion jump) subvolume(s)." [urn:miriam:doi:10.1049/sb:20045021 "Elf J, Ehrenberg M. Spontaneous separation of bi-stable biochemical systems into spatial domains of opposite phases. Systems Biology, IEE Proceedings, volume 1 (2), pages 230-236 (2004)."]
synonym: "Elf algorithm" EXACT []
synonym: "NSM" EXACT []
is_a: KISAO:0000095
disjoint_from: KISAO:0000076
disjoint_from: KISAO:0000074

[Term]
id: KISAO:0000023
name: algorithm using spatial description
namespace: KISAO
def: "Algorithm that takes into account the location of the reacting components." [:]
is_obsolete: true
replaced_by: KISAO:0000000^KISAO:0000245(KISAO:0000102)
creation_date: 2008-07-08T00:00:00Z
created_by: NLN

[Term]
id: KISAO:0000024
name: partial differential equation method
namespace: KISAO
def: "Partial differential equations are used to describe variations in concentrations over both, space and time." [:]
is_obsolete: true
creation_date: 2008-07-08T00:00:00Z
created_by: NLN

[Term]
id: KISAO:0000025
name: Gillespie-like stochastic simulation method
namespace: KISAO
def: "Stochastic simulation algorithm using the an approach alike the one described in Gillespie's papers of 1976 and 1977." [:]
comment: This definition is dodgy, as is the name of the term. That will do for the moment, until we redesign the whole stochastic branch, based on algorithm details.
is_obsolete: true
replaced_by: KISAO:0000241^KISAO:0000245(KISAO:0000104)
creation_date: 2008-07-08T00:00:00Z
created_by: NLN

[Term]
id: KISAO:0000026
name: algorithm using non-spatial description
namespace: KISAO
def: "Algorithms that considers the system to be simulated as made of well-stirred components, that is the activity of the components is the same independently of their location." [:]
is_obsolete: true
creation_date: 2008-07-08T00:00:00Z
created_by: NLN

[Term]
id: KISAO:0000027
name: Gibson-Bruck's next reaction method
namespace: KISAO
def: "As with the first reaction method [KISAO:0000015], a putative reaction time is calculated for each reaction, and the reaction with the shortest reaction time will be realized. However, the unused calculated reaction times are not wasted. The set of reactions is organized in a priority queue to allow for the efficient search for the fastest reaction. In addition, by using a so-called dependency graph only those reaction times are recalculated in each step, that are dependent on the reaction, which has been realized." [urn:miriam:doi:10.1021/jp993732q "Gibson MA, Bruck J. Efficient Exact Stochastic Simulation of Chemical Systems with Many Species and Many Channels. Journal of Physical Chemistry A, Vol. 104, pages 1876-1889 (2000)."]
synonym: "Gibson and Bruck method" EXACT []
is_a: KISAO:0000034
disjoint_from: KISAO:0000003
disjoint_from: KISAO:0000038
disjoint_from: KISAO:0000015
creation_date: 2007-10-10T00:00:00Z
created_by: dk

[Term]
id: KISAO:0000028
name: slow-scale stochastic simulation algorithm
namespace: KISAO
def: "Attempt to overcome the problem of stiff systems by developing an ''approximate theory that allows one to stochastically advance the system in time by simulating the firings of only the slow reaction events''." [urn:miriam:pubmed:15638651 "Cao Y, Gillespie DT, Petzold LR. The slow-scale stochastic simulation algorithm. Journal of Chemical Physics, Vol. 122, No. 1. (1 January 2005)."]
synonym: "slow-scale stochastic SSA" EXACT []
synonym: "ssSSA" EXACT []
is_a: KISAO:0000241
disjoint_from: KISAO:0000039
disjoint_from: KISAO:0000034
disjoint_from: KISAO:0000095
disjoint_from: KISAO:0000097
disjoint_from: KISAO:0000082
disjoint_from: KISAO:0000051
disjoint_from: KISAO:0000029
disjoint_from: KISAO:0000075
relationship: KISAO:0000245 KISAO:0000237

relationship: KISAO:0000247 KISAO:0000102


[Term]
id: KISAO:0000029
name: Gillespie's direct method
namespace: KISAO
def: "Stochastic simulation algorithm using the next-reaction density function, giving the probability that the next reaction will happen in a given time interval. To choose the next reaction to fire, the algorithm directly and separately calculate the identity of the reaction and the time it will fire." [urn:miriam:doi:10.1021/j100540a008 "Gillespie DT. Exact stochastic simulation of coupled chemical reactions. Journal of Physical Chemistry, Vol. 81, No. 25. (1977), pp. 2340-2361."]
synonym: "SSA" EXACT []
synonym: "stochastic simulation algorithm" RELATED []
synonym: "DM" EXACT []
is_a: KISAO:0000241
disjoint_from: KISAO:0000039
disjoint_from: KISAO:0000028
disjoint_from: KISAO:0000034
disjoint_from: KISAO:0000095
disjoint_from: KISAO:0000097
disjoint_from: KISAO:0000082
disjoint_from: KISAO:0000051
disjoint_from: KISAO:0000075
relationship: KISAO:0000245 KISAO:0000236

relationship: KISAO:0000247 KISAO:0000102

creation_date: 2007-10-10T00:00:00Z
created_by: dk

[Term]
id: KISAO:0000030
name: Euler forward method
namespace: KISAO
def: "The Euler method is an explicit one-step method for the numerical integration of ODES with a given initial value. The calculation of the next integration step at time t+1 is based on the state of the system at time point t." [urn:miriam:isbn:052143064X "Press WH, Teukolsky SA, Vetterling WT, Flannery BP. Numerical Recipes. Cambridge University Press, New York, 2nd edition (1992)."]
synonym: "Euler method" EXACT []
is_a: KISAO:0000261
disjoint_from: KISAO:0000031
relationship: KISAO:0000245 KISAO:0000239

creation_date: 2007-10-10T00:00:00Z
created_by: dk

[Term]
id: KISAO:0000031
name: Euler backward method
namespace: KISAO
def: "The Euler backward method is an implicit one-step method for the numerical integration of ODES with a given initial value. The next state of a system is calculated by solving an equation that considers both, the current state of the system and the later one." [urn:miriam:isbn:052143064X "Press WH, Teukolsky SA, Vetterling WT, Flannery BP. Numerical Recipes in Fortran 77. Cambridge University Press (2001)."]
is_a: KISAO:0000261
disjoint_from: KISAO:0000030
relationship: KISAO:0000245 KISAO:0000240

creation_date: 2007-11-02T00:00:00Z
created_by: dk

[Term]
id: KISAO:0000032
name: explicit fourth-order Runge-Kutta method
namespace: KISAO
def: "The Runge-Kutta method is a method for the numerical integration of ODES with a given initial value. The calculation of the next integration step at time t+1 is based on the state of the system at time point t, plus the product of the size of the interval and an estimated slope. The slope is a weighted average of 4 single slope points (beginning of interval-midpoint-midpoint-end of interval)." [urn:miriam:isbn:0-471-91046-5  "Butcher JC. The Numerical Analysis of Ordinary Differential Equations: Runge-Kutta and General Linear Methods (1987). "]
synonym: "RK4" EXACT []
synonym: "Runge-Kutta method" EXACT []
is_a: KISAO:0000064
disjoint_from: KISAO:0000086
disjoint_from: KISAO:0000261
disjoint_from: KISAO:0000033
disjoint_from: KISAO:0000087
relationship: KISAO:0000245 KISAO:0000239

creation_date: 2007-11-12T00:00:00Z
created_by: dk

[Term]
id: KISAO:0000033
name: Rosenbrock method
namespace: KISAO
def: "Some general implicit processes are given for the solution of simultaneous first-order differential equations. These processes, which use successive substitution, are implicit analogues of the (explicit) Runge-Kutta processes. They require the solution in each time step of one or more set of simultaneous linear equations, usually of a special and simple form. Processes of any required order can be devised, and they can be made to have a wide margin of stability when applied to a linear problem." [, urn:miriam:isbn:052143064X "Press WH, Teukolsky SA, Vetterling WT, Flannery BP. Numerical Recipes. Cambridge University Press, New York, 2nd edition, pages 742-746 (1992)."]
comment: The Rosenbrock method is for example used in E-Cell.
synonym: "generalized fourth order runge-kutta method" EXACT []
synonym: "Kaps-Rentrop method" EXACT []
is_a: KISAO:0000064
disjoint_from: KISAO:0000086
disjoint_from: KISAO:0000261
disjoint_from: KISAO:0000087
disjoint_from: KISAO:0000032
relationship: KISAO:0000245 KISAO:0000240

creation_date: 2007-11-12T00:00:00Z
created_by: dk

[Term]
id: KISAO:0000034
name: optimized direct method
namespace: KISAO
def: "Algorithm aimed to speed-up Gillespie's direct method." [:]
is_a: KISAO:0000241
disjoint_from: KISAO:0000039
disjoint_from: KISAO:0000028
disjoint_from: KISAO:0000095
disjoint_from: KISAO:0000097
disjoint_from: KISAO:0000082
disjoint_from: KISAO:0000051
disjoint_from: KISAO:0000029
disjoint_from: KISAO:0000075
relationship: KISAO:0000245 KISAO:0000236

relationship: KISAO:0000247 KISAO:0000102

creation_date: 2008-07-08T00:00:00Z
created_by: NLN

[Term]
id: KISAO:0000035
name: algorithm using deterministic rules
def: "Algorithm that simulates the temporal evolution of a system using determined descriptions, that from a precise initial state always provide the same ending state." [:]
is_obsolete: true
replaced_by: KISAO:0000000^KISAO:0000245(KISAO:0000103)
creation_date: 2008-07-08T00:00:00Z
created_by: NLN

[Term]
id: KISAO:0000036
name: algorithm using stochastic rules
def: "Algorithm that simulates the temporal evolution of a system using probabilistic rules, that from a precise initial state may provide different ending state." [:]
is_obsolete: true
replaced_by: KISAO:0000000^KISAO:0000245(KISAO:0000104)
creation_date: 2008-07-08T00:00:00Z
created_by: NLN

[Term]
id: KISAO:0000037
name: algorithm using fixed timesteps
def: "Algorithm that uses timesteps of constant length to update the state of a system during the whole simulation." [:]
is_obsolete: true
replaced_by: KISAO:0000000^KISAO:0000245(KISAO:0000108)
creation_date: 2008-07-08T00:00:00Z
created_by: NLN

[Term]
id: KISAO:0000038
name: sorting direct method
namespace: KISAO
def: "In order to overcome the problem of high complexity of the Stochastic Simulation Algorithm [KISAO:0000029] when simulating large systems, the sorting direct method maintains a loosely sorted order of the reactions as the simulation executes." [urn:miriam:doi:10.1016/j.compbiolchem.2005.10.007 "McCollum J M, Peterson G D, Cox C D, Simpson M L, Samatova N F. The sorting direct method for stochastic simulation of biochemical systems with varying reaction execution behavior. Computational Biology and Chemistry, Volume 30 (1), pages 39-49 (2006)."]
is_a: KISAO:0000034
disjoint_from: KISAO:0000003
disjoint_from: KISAO:0000027
disjoint_from: KISAO:0000015

[Term]
id: KISAO:0000039
name: tau-leaping method
namespace: KISAO
def: "Approximate acceleration procedure of the Stochastic Simulation Algorithm [KISAO:0000029] that divides the time into subintervals and ''leaps'' from one to another, firing all the reaction events in each subinterval." [urn:miriam:doi:10.1063/1.1378322 "Gillespie DT. Approximate accelerated stochastic simulation of chemically reacting systems. The Journal of Chemical Physics, Vol. 115 (4), pages 1716-1733 (2001). Section V."]
is_a: KISAO:0000241
disjoint_from: KISAO:0000028
disjoint_from: KISAO:0000034
disjoint_from: KISAO:0000095
disjoint_from: KISAO:0000097
disjoint_from: KISAO:0000082
disjoint_from: KISAO:0000051
disjoint_from: KISAO:0000029
disjoint_from: KISAO:0000075
relationship: KISAO:0000245 KISAO:0000237

relationship: KISAO:0000259 KISAO:0000230
cardinality: 1

relationship: KISAO:0000259 KISAO:0000228
cardinality: 1

creation_date: 2008-07-08T00:00:00Z
created_by: NLN

[Term]
id: KISAO:0000040
name: Poisson tau-leaping method
namespace: KISAO
def: "Explicit tau-leaping method with basic preleap check." [urn:miriam:doi:10.1063/1.1378322 "Gillespie DT. Approximate accelerated stochastic simulation of chemically reacting systems. The Journal of Chemical Physics, Vol. 115 (4), pages 1716-1733 (2001). Section V."]
synonym: "explicit tau-leaping method with basic preleap check" EXACT []
synonym: "explicit tau-leaping" EXACT []
synonym: "poisson tau-leaping" EXACT []
is_a: KISAO:0000039
disjoint_from: KISAO:0000046
disjoint_from: KISAO:0000084
disjoint_from: KISAO:0000045
disjoint_from: KISAO:0000081
disjoint_from: KISAO:0000048
disjoint_from: KISAO:0000074
relationship: KISAO:0000245 KISAO:0000239


[Term]
id: KISAO:0000041
name: algorithm using adaptive timesteps
def: "Algorithm that does not use fixed timesteps to update the state of a system during the whole simulation, but on the contrary adapts the length of the timesteps to the local situation." [:]
is_obsolete: true
replaced_by: KISAO:0000000^KISAO:0000245(KISAO:0000107)
creation_date: 2008-07-08T00:00:00Z
created_by: NLN

[Term]
id: KISAO:0000042
name: Non-spatial Gillespie-like method
namespace: KISAO
is_obsolete: true
replaced_by: KISAO:0000241^KISAO:0000247(KISAO:0000102)

[Term]
id: KISAO:0000044
name: Gillespie based method for stiff systems.
namespace: KISAO
is_obsolete: true

[Term]
id: KISAO:0000045
name: implicit tau-leaping based method
namespace: KISAO
def: "Contrary to the (explicit) tau-leaping [KISAO:0000040], the implicit tau-leaping allows for much larger time-steps when simulating stiff systems." [urn:miriam:doi:10.1063/1.1627296 "Rathinam M, Petzold L R, Cao Y, Gillespie D T. Stiffness in stochastic chemically reacting systems: The implicit tau-leaping method. The Journal of Chemical Physics, Volume 119 (24), pages 12784-12794 (2003)."]
is_a: KISAO:0000039
disjoint_from: KISAO:0000046
disjoint_from: KISAO:0000084
disjoint_from: KISAO:0000081
disjoint_from: KISAO:0000040
disjoint_from: KISAO:0000048
disjoint_from: KISAO:0000074
relationship: KISAO:0000259 KISAO:0000248
cardinality: 1

relationship: KISAO:0000245 KISAO:0000240

relationship: KISAO:0000247 KISAO:0000102

creation_date: 2007-10-12T00:00:00Z
created_by: dk

[Term]
id: KISAO:0000046
name: trapezoidal implicit tau-leaping based method
namespace: KISAO
def: "Formula for accelerated discrete efficient stochastic simulation of chemically reacting system [which] has better accuracy and stiff stability properties than the explicit [KISAO:0000079] and implicit [KISAO:0000045] tau-leaping formulas for discrete stochastic systems, and it limits to the trapezoidal rule in the deterministic regime." [citeulike:1755561 "Cao Y, Petzold L. Trapezoidal tau-leaping formula for the stochastic simulation of biochemical systems. Foundations of Systems Biology in Engineering (FOSBE), pages 149-152 (2005)."]
is_a: KISAO:0000039
disjoint_from: KISAO:0000084
disjoint_from: KISAO:0000045
disjoint_from: KISAO:0000081
disjoint_from: KISAO:0000040
disjoint_from: KISAO:0000048
disjoint_from: KISAO:0000074
relationship: KISAO:0000245 KISAO:0000240

relationship: KISAO:0000247 KISAO:0000102

creation_date: 2007-10-16T00:00:00Z
created_by: dk

[Term]
id: KISAO:0000048
name: adaptive explicit-implicit tau-leaping method
namespace: KISAO
def: "Modification of the original tau-selection strategy [KISAO:0000040], designed for explicit tau-leaping, is modified to apply to implicit tau-leaping, allowing for longer steps when the system is stiff. Further, an adaptive strategy is proposed that identifies stiffness and automatically chooses between the explicit and the (new) implicit tau-selection methods to achieve better efficiency." [urn:miriam:doi:10.1063/1.2745299 "Cao Y, Gillespie DT, Petzold LR. Adaptive explicit-implicit tau-leaping method with automatic tau selection. The Journal of Chemical Physics, Vol. 126 (22) (2007)."]
is_a: KISAO:0000039
disjoint_from: KISAO:0000046
disjoint_from: KISAO:0000084
disjoint_from: KISAO:0000045
disjoint_from: KISAO:0000081
disjoint_from: KISAO:0000040
disjoint_from: KISAO:0000074
relationship: KISAO:0000245 KISAO:0000239

relationship: KISAO:0000245 KISAO:0000240

relationship: KISAO:0000247 KISAO:0000102


[Term]
id: KISAO:0000051
name: Bortz-Kalos-Liebowitz method
namespace: KISAO
def: "The Bortz-Kalos-Liebowitz (or: kinetic Monte-Carlo-) method is a stochastic method for the simulation of time evolution of processes using (pseudo-)random numbers." [urn:miriam:doi:10.1016/0021-9991(75)90060-1 "Bortz AB, Kalos MH, Lebowitz JL. A new algorithm for Monte Carlo simulation of Ising spin systems. Journal of Computational Physics, Vol. 17 (1), pages 10-18 (1975)."]
synonym: "BKL" EXACT []
synonym: "n-fold way" EXACT []
synonym: "dynamic monte carlo method" NARROW []
synonym: "KMC" EXACT []
synonym: "kinetic monte carlo method" EXACT []
synonym: "kinetic monte carlo" EXACT []
is_a: KISAO:0000241
disjoint_from: KISAO:0000039
disjoint_from: KISAO:0000028
disjoint_from: KISAO:0000034
disjoint_from: KISAO:0000095
disjoint_from: KISAO:0000097
disjoint_from: KISAO:0000082
disjoint_from: KISAO:0000029
disjoint_from: KISAO:0000075
relationship: KISAO:0000247 KISAO:0000102


[Term]
id: KISAO:0000056
name: Smoluchowski equation based method
namespace: KISAO
def: "Methods based on the Smoluchowski equation." [citeulike:1839950 "Smoluchowski M. Mathematical theory of the kinetics of the coagulation of colloidal solutions. Z. Phys. Chem, Vol. 92, No. 129. (1917)."]
is_a: KISAO:0000000
disjoint_from: KISAO:0000264
disjoint_from: KISAO:0000094
disjoint_from: KISAO:0000241
disjoint_from: KISAO:0000261
disjoint_from: KISAO:0000064
disjoint_from: KISAO:0000017
disjoint_from: KISAO:0000019
disjoint_from: KISAO:0000231
relationship: KISAO:0000245 KISAO:0000104

creation_date: 2007-10-29T00:00:00Z
created_by: dk

[Term]
id: KISAO:0000057
name: Brownian diffusion Smoluchowski method
namespace: KISAO
def: "In the Brownian diffusion Smoluchowski method, ''each molecule is treated as a point-like particle that diffuses freely in three-dimensional space. When a pair of reactive molecules collide, such as an enzyme and its substrate, a reaction occurs and the simulated reactants are replaced by products. [..] Analytic solutions are presented for some simulation parameters while others are calculated using look-up tables''. Supported chemical processes include molecular diffusion, treatment of surfaces, zeroth-order-, unimolecular-, and bimolecular reactions." [urn:miriam:pubmed:16204833 "Andrews SS, Bray D. Stochastic simulation of chemical reactions with spatial resolution and single molecule detail. Phys Biol, volume 1 (3-4), pages 137-151 (December 2004)."]
comment: Used for instance in Smoldyn.
is_a: KISAO:0000056
disjoint_from: KISAO:0000058
relationship: KISAO:0000245 KISAO:0000108

relationship: KISAO:0000259 KISAO:0000258
cardinality: 1

relationship: KISAO:0000245 KISAO:0000102

relationship: KISAO:0000245 KISAO:0000105

relationship: KISAO:0000259 KISAO:0000257
cardinality: 1

relationship: KISAO:0000259 KISAO:0000254
cardinality: 1

relationship: KISAO:0000259 KISAO:0000260
cardinality: 1


[Term]
id: KISAO:0000058
name: GFRD
namespace: KISAO
def: "Method that simulates biochemical networks on particle level. It considers both, changes in time and space by ''exploiting both the exact solution of the Smoluchowski Equation to set up an event-driven algorithm'' which allows for large jumps in time when the considered particles are far away from each other [in space] and thus cannot react. GFRD combines the propagation of particles in space with the reactions taking place between them in one simulation step." [urn:miriam:doi:10.1063/1.2137716 "Van Zon JS, Ten Wolde PR. Green's-function reaction dynamics: A particle-based approach for simulating biochemical networks in time and space. Journal of Chemical Physics, Volume 123 (23) (2005)."]
synonym: "Green's function reaction dynamics" EXACT []
is_a: KISAO:0000056
disjoint_from: KISAO:0000057
relationship: KISAO:0000245 KISAO:0000102

relationship: KISAO:0000245 KISAO:0000105

relationship: KISAO:0000245 KISAO:0000107


[Term]
id: KISAO:0000064
name: Runge-Kutta based method
namespace: KISAO
def: "Explicit or implicit method for the approximation of solutions for ordinary differential equations (ODEs). Runge-Kutta methods have been invented by Runge and Kutta in the 1900s." [urn:miriam:isbn:0-471-91046-5 "Butcher JC. The Numerical Analysis of Ordinary Differential Equations: Runge-Kutta and General Linear Methods (1987)."]
synonym: "modified Euler method" RELATED []
is_a: KISAO:0000000
disjoint_from: KISAO:0000056
disjoint_from: KISAO:0000264
disjoint_from: KISAO:0000094
disjoint_from: KISAO:0000241
disjoint_from: KISAO:0000261
disjoint_from: KISAO:0000017
disjoint_from: KISAO:0000019
disjoint_from: KISAO:0000231
relationship: KISAO:0000245 KISAO:0000108

relationship: KISAO:0000245 KISAO:0000103

relationship: KISAO:0000247 KISAO:0000102

creation_date: 2007-11-12T00:00:00Z
created_by: dk

[Term]
id: KISAO:0000068
name: deterministic cellular automata update algorithm
namespace: KISAO
def: "A cellular automaton is a discrete model of a regular grid of cells with a finite number of dimensions. Each cell has a finite number of defined states. The automaton changes its state in a discrete manner, meaning that the state of a cell at time t is determined by a function of the states of its neighbors at time t - 1. These neighbors are a selection of cells relative to the specified cell. Famous examples for deterministic cellular automata are Conway's game of life or Wolfram's elementary cellular automata." [urn:miriam:isbn:978-0252000232 "Burks, Arthur W (Editor). Essays on Cellular Automata. University of Illinois Press (1970)."]
is_a: KISAO:0000264
disjoint_from: KISAO:0000021
relationship: KISAO:0000245 KISAO:0000103

creation_date: 2007-10-30T00:00:00Z
created_by: dk

[Term]
id: KISAO:0000071
name: LSODE
namespace: KISAO
def: "LSODE solves explicitly given ODE systems. [and] [..] is based on the GEAR and GEARB packages. It solves ODE systems given explicitly as dy/dt = f ( t , y )." [, urn:miriam:doi:10.1145/1218052.1218054 "Hindmarsh AC. LSODE and LSODI, two new initial value ordinary differential equation solvers. SIGNUM Newsletter, Volume 15 (4), pages 10-11 (1980)."]
synonym: "Livermore solver for ordinary differential equations" EXACT []
is_a: KISAO:0000094
disjoint_from: KISAO:0000089
disjoint_from: KISAO:0000088
disjoint_from: KISAO:0000234
disjoint_from: KISAO:0000090
disjoint_from: KISAO:0000232
disjoint_from: KISAO:0000091
disjoint_from: KISAO:0000233
disjoint_from: KISAO:0000093
creation_date: 2007-11-16T00:00:00Z
created_by: dk

[Term]
id: KISAO:0000074
name: binomial tau-leap spatial stochastic simulation algorithm
namespace: KISAO
def: "Coarse grained modified version of the next subvolume method [KISAO:0000022] that allows the user to consider both diffusion and reaction events in relatively long simulation time spans as compared with the original method and other commonly used fully stochastic computational methods." [urn:miriam:doi:10.1063/1.2771548 "Marquez-Lago T., Burrage K. Binomial tau-leap spatial stochastic simulation algorithm for applications in chemical kinetics. The Journal of Chemical Physics, Vol. 127 (10) (2007)."]
is_a: KISAO:0000039
disjoint_from: KISAO:0000076
disjoint_from: KISAO:0000046
disjoint_from: KISAO:0000045
disjoint_from: KISAO:0000022
disjoint_from: KISAO:0000048
disjoint_from: KISAO:0000084
disjoint_from: KISAO:0000040
disjoint_from: KISAO:0000081
relationship: KISAO:0000259 KISAO:0000253
cardinality: 1

creation_date: 2007-10-16T00:00:00Z
created_by: dk

[Term]
id: KISAO:0000075
name: Gillespie-Multi-Particle method
namespace: KISAO
def: "Combination of the multiparticle method for diffusion (Chopard et al. , 1994) and the kinetic Monte Carlo Method [KISAO:0000029]." [urn:miriam:pubmed:16731694 "Rodriguez VJ, Kaandorp JA, Dobrzynski M, Blom JG. Spatial stochastic modelling of the phosphoenolpyruvate-dependent phosphotransferase (PTS) pathway in Escherichia coli. Bioinformatics, Vol. 22 (15), pages 1895-1901 (2006)."]
synonym: "GMP" EXACT []
synonym: "particle-based spatial stochastic method" EXACT []
is_a: KISAO:0000241
disjoint_from: KISAO:0000039
disjoint_from: KISAO:0000028
disjoint_from: KISAO:0000034
disjoint_from: KISAO:0000095
disjoint_from: KISAO:0000097
disjoint_from: KISAO:0000082
disjoint_from: KISAO:0000029
disjoint_from: KISAO:0000051
relationship: KISAO:0000245 KISAO:0000102


[Term]
id: KISAO:0000076
name: Stundzia and Lumsden method
namespace: KISAO
def: "Sub-volume stochastic reaction-diffusion method that using Green's function to link the bulk diffusion coefficient D in Fick's differential law to the corresponding transition rate probability for diffusion of a particle between finite volume elements. This generalized stochastic algorithm enables to numerically calculate the time evolution of a spatially inhomogeneous mixture of reaction-diffusion species in a finite volume. The time step is stochastic and is generated by a probability distribution determined by the intrinsic reaction kinetics and diffusion dynamics." [urn:miriam:doi:10.1006/jcph.1996.0168 "Stundzia AB, Lumsden CJ. Stochastic simulation of coupled reaction-diffusion processes. J Comput Phys, Vol. 127 (1), pages 196-207 (1996)."]
synonym: "reaction-diffusion stochastic simulation algorithm" EXACT []
is_a: KISAO:0000095
disjoint_from: KISAO:0000022
disjoint_from: KISAO:0000074

[Term]
id: KISAO:0000079
name: explicit tau-leaping method
namespace: KISAO
def: "Explicit tau-leaping method." [:]
is_obsolete: true
replaced_by: KISAO:0000039^KISAO:0000245(KISAO:0000239)

[Term]
id: KISAO:0000081
name: explicit tau-leaping method with estimated-mid point technique
namespace: KISAO
def: "Estimated-Midpoint tau-Leap Method: For the selected leaping time tau which satisfies the Leap Condition, compute the expected state change lambda' = tau sumj( aj(x)vj ) during [t, t + tau). Then, with x' =x + [lambda'/2], generate for each j = 1,...,M a sample value kj of the Poisson random variable P(aj(x'), tau). Compute the actual state change, lambda = sumj( kjvj ), and effect the leap by replacing t by t + tau and x by x + lambda." [urn:miriam:doi:10.1063/1.1378322 "Gillespie DT. Approximate accelerated stochastic simulation of chemically reacting systems. The Journal of Chemical Physics, Vol. 115 (4), pages 1716-1733 (2001). Section VI."]
is_a: KISAO:0000039
disjoint_from: KISAO:0000046
disjoint_from: KISAO:0000084
disjoint_from: KISAO:0000045
disjoint_from: KISAO:0000040
disjoint_from: KISAO:0000048
disjoint_from: KISAO:0000074
relationship: KISAO:0000245 KISAO:0000239


[Term]
id: KISAO:0000082
name: k-alpha leaping method
namespace: KISAO
def: "Alternative to the tau-leaping [KISAO:0000039], where one leaps a fixed number of reaction-events." [urn:miriam:doi:10.1063/1.1378322 "Gillespie DT. Approximate accelerated stochastic simulation of chemically reacting systems. The Journal of Chemical Physics, Vol. 115 (4), pages 1716-1733 (2001). Section VIII."]
is_a: KISAO:0000241
disjoint_from: KISAO:0000039
disjoint_from: KISAO:0000028
disjoint_from: KISAO:0000034
disjoint_from: KISAO:0000095
disjoint_from: KISAO:0000097
disjoint_from: KISAO:0000029
disjoint_from: KISAO:0000051
disjoint_from: KISAO:0000075
relationship: KISAO:0000245 KISAO:0000237


[Term]
id: KISAO:0000083
name: implicit tau-leaping method
namespace: KISAO
def: "Implicit tau-leaping method." [:]
is_obsolete: true
replaced_by: KISAO:0000039^KISAO:0000245(KISAO:0000240)

[Term]
id: KISAO:0000084
name: nonnegative Poisson tau-leaping method
namespace: KISAO
def: "The explicit tau-leaping procedure attempts to speed up the stochastic simulation of a chemically reacting system by approximating the number of firings of each reaction channel during a chosen time increment Tau as a Poisson random variable. Since the Poisson random variable can have arbitrarily large sample values, there is always the possibility that this procedure will cause one or more reaction channels to fire so many times during Tau that the population of some reactant species will be driven negative. Two recent papers have shown how that unacceptable occurrence can be avoided by replacing the Poisson random variables with binomial random variables, whose values are naturally bounded. This paper describes a modified Poisson tau-leaping procedure that also avoids negative populations, but is easier to implement than the binomial procedure. The new Poisson procedure also introduces a second control parameter, whose value essentially dials the procedure from the original Poisson tau-leaping at one extreme to the exact stochastic simulation algorithm at the other; therefore, the modified Poisson procedure will generally be more accurate than the original Poisson procedure." [urn:miriam:doi:10.1063/1.1992473 "Cao Y, Gillespie DT, Petzold LR. Avoiding negative populations in explicit Poisson tau-leaping. Journal of Chemical Physics, Vol. 123, 4104 (2005)."]
synonym: "modified poisson tau-leaping" RELATED []
is_a: KISAO:0000039
disjoint_from: KISAO:0000046
disjoint_from: KISAO:0000045
disjoint_from: KISAO:0000081
disjoint_from: KISAO:0000040
disjoint_from: KISAO:0000048
disjoint_from: KISAO:0000074
relationship: KISAO:0000245 KISAO:0000239

relationship: KISAO:0000259 KISAO:0000249
cardinality: 1


[Term]
id: KISAO:0000086
name: Runge-Kutta-Fehlberg based method
namespace: KISAO
def: "The method was developed by the German mathematician Erwin Fehlberg and is based on the class of Runge-Kutta methods. The Runge-Kutta-Fehlberg method uses an O(h4) method together with an O(h5) method that uses all of the points of the O(h4) method, and hence is often referred to as an RKF45 method. Similar schemes with different orders have since been developed. By performing one extra calculation that would be required for an RK5 method, the error in the solution can be estimated and controlled and an appropriate step size can be determined automatically, making this method efficient for ordinary problems of automated numerical integration of ordinary differential equations." [, urn:miriam:pubmed:14990450 "Takahashi K, Kaizu K, Hu B, Tomita M. A multi-algorithm, multi-timescale method for cell simulation. Bioinformatics volume 20(4), pages 538-46 (2004)."]
comment: As used in E-Cell.
synonym: "RKF45" EXACT []
synonym: "Fehlberg method" EXACT []
is_a: KISAO:0000064
disjoint_from: KISAO:0000261
disjoint_from: KISAO:0000033
disjoint_from: KISAO:0000087
disjoint_from: KISAO:0000032

[Term]
id: KISAO:0000087
name: Dormand-Prince 5(4) based method
namespace: KISAO
def: "Dormand-Prince is an explicit method for the numerical integration of ODES with a given initial value." [, urn:miriam:pubmed:14990450 "Takahashi K, Kaizu K, Hu B, Tomita M. A multi-algorithm, multi-timescale method for cell simulation. Bioinformatics volume 20(4), pages 538-46 (2004)."]
comment: As used, for example, in Matlab or in ECell3.
synonym: "DP45" EXACT []
is_a: KISAO:0000064
disjoint_from: KISAO:0000086
disjoint_from: KISAO:0000261
disjoint_from: KISAO:0000033
disjoint_from: KISAO:0000032
creation_date: 2007-11-12T00:00:00Z
created_by: dk

[Term]
id: KISAO:0000088
name: LSODA
namespace: KISAO
def: "LSODA was written by Linda R Petzold and Alan C Hindmarsh. It solves systems dy/dt = f with a dense or banded Jacobian when the problem is stiff, but it automatically selects between non-stiff (Adams) and stiff (BDF) methods. It uses the non-stiff method initially, and dynamically monitors data in order to decide which method to use." [, urn:miriam:doi:10.1137/0904010 "Petzold LR. Automatic Selection of Methods for Solving Stiff and Nonstiff Systems of Ordinary Differential Equations. SIAM Journal on Scientific and Statistical Computing, Vol. 4 (1), pages 136-148 (1983)."]
synonym: "Livermore solver for ordinary differential equations with automatic method switching" EXACT []
is_a: KISAO:0000094
disjoint_from: KISAO:0000089
disjoint_from: KISAO:0000234
disjoint_from: KISAO:0000071
disjoint_from: KISAO:0000090
disjoint_from: KISAO:0000232
disjoint_from: KISAO:0000091
disjoint_from: KISAO:0000233
disjoint_from: KISAO:0000093
relationship: KISAO:0000259 KISAO:0000220
cardinality: 1

relationship: KISAO:0000259 KISAO:0000219
cardinality: 1

creation_date: 2007-10-30T00:00:00Z
created_by: dk

[Term]
id: KISAO:0000089
name: LSODAR
namespace: KISAO
def: "LSODAR, written jointly with L. R. Petzold, is a variant of LSODA with a rootfinding capability added. Thus it solves problems dy/dt = f with dense or banded Jacobian and automatic method selection, and at the same time, it finds the roots of any of a set of given functions of the form g(t,y). This is often useful for finding stop conditions, or for finding points at which a switch is to be made in the function f. The LSODAR source is commented extensively to facilitate modification. Both a single-precision version and a double-precision version are available." [, http://www.nea.fr/abs/html/uscd1228.html "Petzold LR, Hindmarsh, AC. LSODAR: Livermore solver of ordinary differential equations with automatic method switching and root finding, Computing and Mathematics Research Division, 1-316 Lawerence Livermore National Laboratory (1987)."]
synonym: "Livermore solver for ordinary differential equations with automatic method switching and root finding" EXACT []
synonym: "ordinary differential equation solver for stiff or non-stiff systems with root finding" EXACT []
is_a: KISAO:0000094
disjoint_from: KISAO:0000088
disjoint_from: KISAO:0000234
disjoint_from: KISAO:0000071
disjoint_from: KISAO:0000090
disjoint_from: KISAO:0000232
disjoint_from: KISAO:0000091
disjoint_from: KISAO:0000233
disjoint_from: KISAO:0000093
creation_date: 2007-10-27T00:00:00Z
created_by: dk

[Term]
id: KISAO:0000090
name: LSODI
namespace: KISAO
def: "LSODI solves systems given in linearly implicit form, including differential-algebraic systems." [, http://www.nea.fr/abs/html/uscd1224.html ""]
synonym: "Livermore solver for ordinary differential equations, implicit version" EXACT []
is_a: KISAO:0000094
disjoint_from: KISAO:0000089
disjoint_from: KISAO:0000088
disjoint_from: KISAO:0000234
disjoint_from: KISAO:0000071
disjoint_from: KISAO:0000232
disjoint_from: KISAO:0000091
disjoint_from: KISAO:0000233
disjoint_from: KISAO:0000093

[Term]
id: KISAO:0000091
name: LSODIS
namespace: KISAO
def: "LSODIS is a set of general-purpose FORTRAN routines solver for the initial value problem for ordinary differential equation systems. It is suitable for both stiff and nonstiff systems. LSODIS treat systems in the linearly implicit form A(t,y) dy/dt = g(t,y), A = a square matrix, i.e. with the derivative dy/dt implicit, but linearly so." [, http://www.nea.fr/abs/html/uscd1225.html "Seager M, Balsdon S. LSODIS - A sparse implicit ODE solver. 10th World Congress on System Simulation and Scientific Computation, pages 437-439 (1983)."]
synonym: "Livermore solver for ordinary differential equations, implicit sparse version" EXACT []
is_a: KISAO:0000094
disjoint_from: KISAO:0000089
disjoint_from: KISAO:0000088
disjoint_from: KISAO:0000234
disjoint_from: KISAO:0000071
disjoint_from: KISAO:0000090
disjoint_from: KISAO:0000232
disjoint_from: KISAO:0000233
disjoint_from: KISAO:0000093
creation_date: 2007-10-30T00:00:00Z
created_by: dk

[Term]
id: KISAO:0000093
name: LSODPK
namespace: KISAO
def: "LSODPK, written jointly with Peter N Brown, is a set of FORTRAN subroutines for solving the initial value problem for stiff and nonstiff systems of ordinary differential equations. In solving stiff systems, LSODPK uses a corrector iteration composed of Newton iteration and one of four preconditoned Krylov subspace iteration methods. The user must select the desired Krylov method and supply a pair of routine to evaluate, preprocess, and solve the (left and/or right) preconditioner matrices. Aside from preconditioning, the implementation is matrix-free, meaning that explicit storage of the Jacobian (or related) matrix is not required. The method is experimental because the scope of problems for which it is effective is not well-known, and users are forewarned that LSODPK may or may not be competitive with traditional methods on a given problem. LSODPK also includes an option for a user-supplied linear system solver to be used without Krylov iteration." [, http://www.nea.fr/abs/html/uscd1231.html ""]
synonym: "Livermore solver for ordinary differential equations for stiff and nonstiff systems with krylov corrector iteration" EXACT []
synonym: "Livermore solver for ordinary differential equations for stiff and nonstiff systems with Krylov corrector iteration" RELATED []
is_a: KISAO:0000094
disjoint_from: KISAO:0000089
disjoint_from: KISAO:0000088
disjoint_from: KISAO:0000234
disjoint_from: KISAO:0000071
disjoint_from: KISAO:0000090
disjoint_from: KISAO:0000232
disjoint_from: KISAO:0000091
disjoint_from: KISAO:0000233
creation_date: 2008-07-08T00:00:00Z
created_by: NLN

[Term]
id: KISAO:0000094
name: Livermore solver
namespace: KISAO
def: "Method to solve ordinary differential equations developed at the Lawrence Livermore National Laboratory." [:]
is_a: KISAO:0000000
disjoint_from: KISAO:0000056
disjoint_from: KISAO:0000264
disjoint_from: KISAO:0000241
disjoint_from: KISAO:0000261
disjoint_from: KISAO:0000064
disjoint_from: KISAO:0000017
disjoint_from: KISAO:0000019
disjoint_from: KISAO:0000231
relationship: KISAO:0000245 KISAO:0000103

relationship: KISAO:0000247 KISAO:0000102

relationship: KISAO:0000245 KISAO:0000107

relationship: KISAO:0000245 KISAO:0000106

creation_date: 2008-07-08T00:00:00Z
created_by: NLN

[Term]
id: KISAO:0000095
name: sub-volume stochastic reaction-diffusion algorithm
namespace: KISAO
def: "Stochastic method using a combination of discretisation of compartment volumes into voxels and Gillespie-like algorithm to simulate the evolution of the system." [:]
is_a: KISAO:0000241
disjoint_from: KISAO:0000039
disjoint_from: KISAO:0000028
disjoint_from: KISAO:0000034
disjoint_from: KISAO:0000097
disjoint_from: KISAO:0000082
disjoint_from: KISAO:0000029
disjoint_from: KISAO:0000051
disjoint_from: KISAO:0000075
relationship: KISAO:0000245 KISAO:0000102

creation_date: 2008-07-08T00:00:00Z
created_by: NLN

[Term]
id: KISAO:0000096
name: Gillespie-like exact stochastic simulation method
namespace: KISAO
def: "Gillespie-like algorithm that produces exact realisation of the vector of entity amounts at each time by choosing rigorously time and reaction at each iteration." [:]
is_obsolete: true
replaced_by: KISAO:0000241^KISAO:0000245(KISAO:0000236)^KISAO:0000245(KISAO:0000104)
created_by: NLN
creation_date: 2008-07-14T00:00:00Z

[Term]
id: KISAO:0000097
name: kinetic simulation algorithm characteristic
namespace: KISAO
def: "Simulation algorithm property, which can for example describe the model, such as the type of variables (discrete or continuous), and information on the treatment of spatial descriptions, or can be a numerical characteristic, such as the system's behavior (deterministic or stochastic) as well as the progression mechanism (fixed or adaptive time steps)." [:]
disjoint_from: KISAO:0000039
disjoint_from: KISAO:0000028
disjoint_from: KISAO:0000034
disjoint_from: KISAO:0000201
disjoint_from: KISAO:0000095
disjoint_from: KISAO:0000000
disjoint_from: KISAO:0000082
disjoint_from: KISAO:0000029
disjoint_from: KISAO:0000051
disjoint_from: KISAO:0000075
created_by: AZ

[Term]
id: KISAO:0000098
name: type of variable
namespace: KISAO
def: "Type of variables used for the simulation." [:]
is_a: KISAO:0000097
disjoint_from: KISAO:0000102
disjoint_from: KISAO:0000238
disjoint_from: KISAO:0000235
disjoint_from: KISAO:0000099
disjoint_from: KISAO:0000100

[Term]
id: KISAO:0000099
name: type of system behaviour
namespace: KISAO
def: "Characteristic describind the rules, algorithm uses to simulate the temporal evolution of a system: if it may provide different or always the same ending state from a precise initial one." [:]
is_a: KISAO:0000097
disjoint_from: KISAO:0000102
disjoint_from: KISAO:0000238
disjoint_from: KISAO:0000235
disjoint_from: KISAO:0000098
disjoint_from: KISAO:0000100

[Term]
id: KISAO:0000100
name: type of progression time step
namespace: KISAO
def: "Type of time steps used by the algorithm." [:]
is_a: KISAO:0000097
disjoint_from: KISAO:0000102
disjoint_from: KISAO:0000238
disjoint_from: KISAO:0000235
disjoint_from: KISAO:0000098
disjoint_from: KISAO:0000099

[Term]
id: KISAO:0000102
name: spatial description
namespace: KISAO
def: "Algorithm that takes into account the location of the reacting components." [:]
is_a: KISAO:0000097
disjoint_from: KISAO:0000238
disjoint_from: KISAO:0000235
disjoint_from: KISAO:0000098
disjoint_from: KISAO:0000099
disjoint_from: KISAO:0000100
creation_date: 2008-07-08T00:00:00Z
created_by: NLN

[Term]
id: KISAO:0000103
name: deterministic system behaviour
namespace: KISAO
def: "Algorithm that simulates the temporal evolution of a system using determined descriptions, that from a precise initial state always provide the same ending state." [:]
is_a: KISAO:0000099
disjoint_from: KISAO:0000104
creation_date: 2008-07-08T00:00:00Z
created_by: NLN

[Term]
id: KISAO:0000104
name: stochastic system behaviour
namespace: KISAO
def: "Algorithm that simulates the temporal evolution of a system using probabilistic rules, that from a precise initial state may provide different ending state." [:]
is_a: KISAO:0000099
disjoint_from: KISAO:0000103
creation_date: 2008-07-08T00:00:00Z
created_by: NLN

[Term]
id: KISAO:0000105
name: discrete variable
namespace: KISAO
def: "Algorithm that allows to change the values of a system's variables by discrete (integral) amounts." [:]
is_a: KISAO:0000098
disjoint_from: KISAO:0000106
creation_date: 2008-07-08T00:00:00Z
created_by: NLN

[Term]
id: KISAO:0000106
name: continuous variable
namespace: KISAO
def: "Algorithm that allows to change the values of a system's variables by continuous (non-integral) amounts." [:]
is_a: KISAO:0000098
disjoint_from: KISAO:0000105
creation_date: 2008-07-08T00:00:00Z
created_by: NLN

[Term]
id: KISAO:0000107
name: progression with adaptive time step
namespace: KISAO
def: "Algorithm that does not use fixed timesteps to update the state of a system during the whole simulation, but on the contrary adapts the length of the timesteps to the local situation." [:]
is_a: KISAO:0000100
disjoint_from: KISAO:0000108
creation_date: 2008-07-08T00:00:00Z
created_by: NLN

[Term]
id: KISAO:0000108
name: progression with fixed time step
namespace: KISAO
def: "Algorithm that uses timesteps of constant length to update the state of a system during the whole simulation." [:]
is_a: KISAO:0000100
disjoint_from: KISAO:0000107
creation_date: 2008-07-08T00:00:00Z
created_by: NLN

[Term]
id: KISAO:0000114
name: step size fraction
namespace: KISAO
def: "The step size fraction is a floating-point number specifying the step size, as a fraction of the total time range for the simulation. The 'step size fraction' is only enabled for ODE-based deterministic simulators. If you are using a simulator with a fixed step-size, the simulator will use your step size as the fixed step size for the entire time interval. If you are using a simulator with an adaptive step-size, the simulator will use this step size for the initial time-step; it will change the step size for time steps after the initial time step, depending on the error control parameters. For fixed step-size simulators, if you specify a step size fraction that is too large, the simulator may exceed its error threshold, in which case the simulation will halt with an exception (and it will suggest that you re-run the simulation with a large minimum number of time steps). If you are using a stochastic Tau-Leap simulator, the step-size fraction specifies the maximum the ratio of the reaction time scale to the ''leap'' time scale. (If the ''leap'' time scale gets too small, the simulator will revert to stepping with the Gibson-Bruck algorithm) [Dizzy Userguide]." [:]
is_a: KISAO:0000244
disjoint_from: KISAO:0000213
disjoint_from: KISAO:0000223
disjoint_from: KISAO:0000253
relationship: KISAO:0000250 KISAO:0000000^KISAO:0000245(KISAO:0000103)


[Term]
id: KISAO:0000201
name: kinetic simulation algorithm parameter
namespace: KISAO
def: "Parameter that can be used in the simulation experiment settings." [:]
disjoint_from: KISAO:0000000
disjoint_from: KISAO:0000097
relationship: KISAO:0000250 KISAO:0000000

created_by: AZ

[Term]
id: KISAO:0000203
name: particle number lower limit
namespace: KISAO
def: "This parameter is a double value specifying the lower limit for particle numbers. Species with a particle number below this value are considered as having a low particle number. The 'particle number lower limit' cannot be higher than the 'particle number upper limit'. The default value is 800 [COPASI Userguide]." [:]
is_a: KISAO:0000252
disjoint_from: KISAO:0000249
disjoint_from: KISAO:0000204
disjoint_from: KISAO:0000205
disjoint_from: KISAO:0000260
disjoint_from: KISAO:0000258
disjoint_from: KISAO:0000248
disjoint_from: KISAO:0000257
relationship: KISAO:0000250 KISAO:0000231


[Term]
id: KISAO:0000204
name: particle number upper limit
namespace: KISAO
def: "This parameter is a double value specifying the upper limit for particle numbers. Species with a particle number above this value are considered as having a high particle number. The 'particle number upper limit' cannot be lower than the 'particle number lower limit'. The default value is 1000 [COPASI Userguide]." [:]
is_a: KISAO:0000252
disjoint_from: KISAO:0000249
disjoint_from: KISAO:0000203
disjoint_from: KISAO:0000205
disjoint_from: KISAO:0000260
disjoint_from: KISAO:0000258
disjoint_from: KISAO:0000248
disjoint_from: KISAO:0000257
relationship: KISAO:0000250 KISAO:0000231


[Term]
id: KISAO:0000205
name: partitioning interval
namespace: KISAO
def: "This positive integer value specifies after how many steps the internal partitioning of the system should be recalculated. The default is 1, i.e. after every step the partitioning of the system is checked [COPASI Userguide]." [:]
is_a: KISAO:0000252
disjoint_from: KISAO:0000249
disjoint_from: KISAO:0000204
disjoint_from: KISAO:0000203
disjoint_from: KISAO:0000260
disjoint_from: KISAO:0000258
disjoint_from: KISAO:0000248
disjoint_from: KISAO:0000257
relationship: KISAO:0000250 KISAO:0000000^KISAO:0000246(KISAO:0000000)


[Term]
id: KISAO:0000209
name: relative tolerance
namespace: KISAO
def: "This parameter is a numeric value specifying the desired relative tolerance the user wants to achieve. A smaller value means that the trajectory is calculated more accurate. The default value is 1.0 * 10^-6. Please note that best achievable relative tolerance is approximately 2.22 * 10^-16 [COPASI Userguide]. " [:]
is_a: KISAO:0000242
disjoint_from: KISAO:0000254
disjoint_from: KISAO:0000211
disjoint_from: KISAO:0000228

[Term]
id: KISAO:0000211
name: absolute tolerance
namespace: KISAO
def: "This parameter is a positive numeric value specifying the desired absolute tolerance the user wants to achieve. Please note that for species the absolute tolerance is applied to the concentration value. The default value is 1.0 * 10^-12 [COPASI Userguide]." [:]
is_a: KISAO:0000242
disjoint_from: KISAO:0000254
disjoint_from: KISAO:0000209
disjoint_from: KISAO:0000228

[Term]
id: KISAO:0000213
name: Runge-Kutta step size (hybrid)
namespace: KISAO
def: "This positive double value is the step size of the Runge-Kutta solver for the integration of the deterministic part of the system. The default value is 0.001 [COPASI Userguide]." [:]
is_a: KISAO:0000244
disjoint_from: KISAO:0000223
disjoint_from: KISAO:0000253
disjoint_from: KISAO:0000114
relationship: KISAO:0000250 KISAO:0000064


[Term]
id: KISAO:0000216
name: integrate reduced model
namespace: KISAO
def: "This parameter is a boolean value to determine whether the integration shall be performed using the mass conservation laws, i.e., reducing the number of system variables or to use the complete model. A value of 1 (the default) instructs COPASI to make use of the mass conservation laws, whereas a value of 0 instructs COPASI to determine all variables through ODEs [COPASI Userguide]." [:]
is_a: KISAO:0000243
disjoint_from: KISAO:0000220
disjoint_from: KISAO:0000230
disjoint_from: KISAO:0000219

[Term]
id: KISAO:0000219
name: LSODA maximum non-stiff order
namespace: KISAO
def: "This parameter is a positive integer value specifying the maximal order the non-stiff Adams integration method shall attempt before switching to the stiff BDF method. The default and maximal order is 12 [COPASI Userguide]." [:]
synonym: "Adams max order" NARROW []
is_a: KISAO:0000243
disjoint_from: KISAO:0000216
disjoint_from: KISAO:0000220
disjoint_from: KISAO:0000230
relationship: KISAO:0000250 KISAO:0000088


[Term]
id: KISAO:0000220
name: LSODA maximum stiff order
namespace: KISAO
def: "This parameter is a positive integer value specifying the maximal order the stiff BDF integration method shall attempt before switching to smaller internal step sizes. The default and maximal order is 5 [COPASI Userguide]." [:]
synonym: "BDF max order" NARROW []
is_a: KISAO:0000243
disjoint_from: KISAO:0000216
disjoint_from: KISAO:0000230
disjoint_from: KISAO:0000219
relationship: KISAO:0000250 KISAO:0000088


[Term]
id: KISAO:0000223
name: number of history bins
namespace: KISAO
def: "The 'number of history bins' is only enabled for models that contain delayed or multistep reactions for specifying the granularity with which the delayed reaction solver should retain the history of species values, for species that participate in delayed reactions. The default value is 400. The minimum value is 10. If you are having trouble with mass conservation in an ODE simulation of a model with a delayed reaction, try increasing this parameter [Dizzy Userguide]. " [:]
is_a: KISAO:0000244
disjoint_from: KISAO:0000213
disjoint_from: KISAO:0000253
disjoint_from: KISAO:0000114

[Term]
id: KISAO:0000228
name: tau-leaping epsilon
namespace: KISAO
def: "The leap condition is chosen such that the expected change in the propensity function aj(x) is bounded by Epsilon * a0 where Epsilon is an error control parameter between 0 and 1. This parameter is the basic error control mechanism for the Tau-Leaping algorithm. As Epsilon decreases the leaps become shorter and the simulation is more accurate." [urn:miriam:doi:10.1063/1.1378322 "Gillespie DT. Approximate accelerated stochastic simulation of chemically reacting systems. The Journal of Chemical Physics, Vol. 115 (4), pages 1716-1733 (2001). Section V."]
synonym: "tolerance" RELATED []
is_a: KISAO:0000242
disjoint_from: KISAO:0000254
disjoint_from: KISAO:0000209
disjoint_from: KISAO:0000211
relationship: KISAO:0000250 KISAO:0000039


[Term]
id: KISAO:0000230
name: minimum reactions per leap
namespace: KISAO
def: "The tau-leaping driver adaptively switches to the SSA Direct Method when the number of reactions in a single tau-leaping leap step is less than the threshold. By default, this value is 10 [StochKit Userguide]." [:]
synonym: "threshold" RELATED []
is_a: KISAO:0000243
disjoint_from: KISAO:0000220
disjoint_from: KISAO:0000216
disjoint_from: KISAO:0000219
relationship: KISAO:0000250 KISAO:0000039


[Term]
id: KISAO:0000231
name: Pahle hybrid method
namespace: KISAO
def: "The hybrid method combines the stochastic 'Gibson-Bruck's next reaction method' with different algorithms for the numerical integration of ODEs. The biochemical network is dynamically partitioned into a deterministic and a stochastic subnet depending on the current particle numbers in the system. The user can define limits for when a particle number should be considered low or high. The stochastic subnet contains reactions involving low numbered species as substrate or product. All the other reactions form the deterministic subnet. The two subnets are then simulated in parallel using the stochastic and deterministic solver, respectively. The reaction probabilities in the stochastic subnet are approximated as constant between two stochastic reaction events." [urn:miriam:pubmed:17032683 "Pahle,J. (2002) Eine Hybridmethode zur Simulation biochemischer Prozess (in German). Diploma thesis Universita Karlsruhe (TH), Germany., COPASI--a COmplex PAthway SImulator. Hoops S, Sahle S, Gauges R, Lee C, Pahle J, Simus N, Singhal M, Xu L, Mendes P, Kummer U. Bioinformatics. 2006 Dec 15;22(24):3067-74. Epub 2006 Oct 10."]
is_a: KISAO:0000000
disjoint_from: KISAO:0000056
disjoint_from: KISAO:0000264
disjoint_from: KISAO:0000094
disjoint_from: KISAO:0000241
disjoint_from: KISAO:0000261
disjoint_from: KISAO:0000064
disjoint_from: KISAO:0000017
disjoint_from: KISAO:0000019
relationship: KISAO:0000259 KISAO:0000203
cardinality: 1

relationship: KISAO:0000245 KISAO:0000103

relationship: KISAO:0000259 KISAO:0000204
cardinality: 1

relationship: KISAO:0000245 KISAO:0000104

relationship: KISAO:0000246 KISAO:0000088

relationship: KISAO:0000246 KISAO:0000027

created_by: AZ

[Term]
id: KISAO:0000232
name: LSOIBT
def: "LSOIBT is a set of general-purpose FORTRAN routines solver for the initial value problem for ordinary differential equation systems. It is suitable for both stiff and nonstiff systems. LSOIBT treat systems in the linearly implicit form A(t,y) dy/dt = g(t,y), A = a square matrix, i.e. with the derivative dy/dt implicit, but linearly so. It allows A to be singular, in which case the system is a differential-algebraic equation (DAE) system. In that case, the user must be very careful to supply a well-posed problem with consistent initial conditions. LSOIBT, written jointly with C. S. Kenney, solves linearly implicit systems in which the matrices involved are all assumed to be block-tridiagonal. Linear systems are solved by the LU method. The LSOIBT source is commented extensively to facilitate modification. Both a single-precision version and a double-precision version are available." [, http://www.nea.fr/abs/html/uscd1226.html ""]
synonym: "Livermore solver for ordinary differential equations given in implicit form, with block-tridiagonal Jacobian treatment" EXACT []
is_a: KISAO:0000094
disjoint_from: KISAO:0000089
disjoint_from: KISAO:0000088
disjoint_from: KISAO:0000234
disjoint_from: KISAO:0000071
disjoint_from: KISAO:0000090
disjoint_from: KISAO:0000091
disjoint_from: KISAO:0000233
disjoint_from: KISAO:0000093

[Term]
id: KISAO:0000233
name: LSODES
def: "LSODES, written jointly with A. H. Sherman, solves systems dy/dt = f and in the stiff case treats the Jacobian matrix in general sparse form. It determines the sparsity structure on its own, or optionally accepts this information from the user. It then uses parts of the Yale Sparse Matrix Package (YSMP) to solve the linear systems that arise, by a sparse (direct) LU factorization/backsolve method. The LSODES source is commented extensively to facilitate modification. Both a single-precision version and a double-precision version are available." [, http://www.nea.fr/abs/html/uscd1229.html ""]
synonym: "Livermore solver for ordinary differential equations with general sparse Jacobian matrix" EXACT []
is_a: KISAO:0000094
disjoint_from: KISAO:0000089
disjoint_from: KISAO:0000088
disjoint_from: KISAO:0000234
disjoint_from: KISAO:0000071
disjoint_from: KISAO:0000090
disjoint_from: KISAO:0000232
disjoint_from: KISAO:0000091
disjoint_from: KISAO:0000093

[Term]
id: KISAO:0000234
name: LSODKR
def: "LSODKR is a new initial value ODE solver for stiff and nonstiff systems. It is a variant of the LSODPK and LSODE solvers, intended mainly for large stiff systems. The main differences between LSODKR and LSODE are the following: a) for stiff systems, LSODKR uses a corrector iteration composed of Newton iteration and one of four preconditioned Krylov subspace iteration methods. The user must supply routines for the preconditioning operations, b) within the corrector iteration, LSODKR does automatic switching between functional (fixpoint) iteration and modified Newton iteration, c) LSODKR includes the ability to find roots of given functions of the solution during the integration." [, http://www.nea.fr/abs/html/uscd1230.html ""]
synonym: "Livermore solver for ordinary differential equations, with preconditioned Krylov iteration methods for the Newton correction linear systems, and with root finding." EXACT []
is_a: KISAO:0000094
disjoint_from: KISAO:0000089
disjoint_from: KISAO:0000088
disjoint_from: KISAO:0000071
disjoint_from: KISAO:0000090
disjoint_from: KISAO:0000232
disjoint_from: KISAO:0000233
disjoint_from: KISAO:0000091
disjoint_from: KISAO:0000093

[Term]
id: KISAO:0000235
name: type of solution
namespace: KISAO
def: "Characteristic describing if the solution produced by the method is exact or approximate." [:]
is_a: KISAO:0000097
disjoint_from: KISAO:0000102
disjoint_from: KISAO:0000238
disjoint_from: KISAO:0000098
disjoint_from: KISAO:0000099
disjoint_from: KISAO:0000100

[Term]
id: KISAO:0000236
name: exact solution
namespace: KISAO
def: "Algorithms providing exact solution." [:]
is_a: KISAO:0000235
disjoint_from: KISAO:0000237

[Term]
id: KISAO:0000237
name: approximate solution
namespace: KISAO
def: "Approximation algorithms are algorithms used to find approximate solutions to optimization problems. Approximation algorithms are often associated with NP-hard problems; since it is unlikely that there can ever be efficient polynomial time exact algorithms solving NP-hard problems, one settles for polynomial time sub-optimal solutions. Unlike heuristics, which usually only find reasonably good solutions reasonably fast, one wants provable solution quality and provable run time bounds. Ideally, the approximation is optimal up to a small constant factor (for instance within 5% of the optimal solution). Approximation algorithms are increasingly being used for problems where exact polynomial-time algorithms are known but are too expensive due to the input size." [:]
is_a: KISAO:0000235
disjoint_from: KISAO:0000236

[Term]
id: KISAO:0000238
name: type of method
namespace: KISAO
def: "Characteristic, describing if the method finds a solution by solving an equation involving only the current state of the system (explicit) or both the current and the later one (implicit). " [:]
is_a: KISAO:0000097
disjoint_from: KISAO:0000102
disjoint_from: KISAO:0000235
disjoint_from: KISAO:0000098
disjoint_from: KISAO:0000099
disjoint_from: KISAO:0000100

[Term]
id: KISAO:0000239
name: explicit method type
namespace: KISAO
def: "Explicit methods calculate the state of a system at a later time from the state of the system at the current time. Mathematically, if Y(t) is the current system state and Y((t+delta t) is the state at the later time (delta t is a small time step), then, for an explicit method Y(t+delta t) = F(Y(t)), to find Y(t+delta t)." [:]
is_a: KISAO:0000238
disjoint_from: KISAO:0000240

[Term]
id: KISAO:0000240
name: implicit method type
namespace: KISAO
def: "Implicit methods find a solution by solving an equation involving both the current state of the system and the later one. Mathematically, if Y(t) is the current system state and Y((t+delta t) is the state at the later time (delta t is a small time step), then, for an implicit method one solves an equation G(Y(t), Y(t+delta t))=0, to find Y(t+delta t)." [:]
is_a: KISAO:0000238
disjoint_from: KISAO:0000239

[Term]
id: KISAO:0000241
name: Gillespie-like method
def: "Stochastic simulation algorithm using the an approach alike the one described in Gillespie's papers of 1976 and 1977." [:]
is_a: KISAO:0000000
disjoint_from: KISAO:0000056
disjoint_from: KISAO:0000264
disjoint_from: KISAO:0000094
disjoint_from: KISAO:0000261
disjoint_from: KISAO:0000064
disjoint_from: KISAO:0000017
disjoint_from: KISAO:0000019
disjoint_from: KISAO:0000231
relationship: KISAO:0000245 KISAO:0000105

relationship: KISAO:0000245 KISAO:0000104

relationship: KISAO:0000245 KISAO:0000107


[Term]
id: KISAO:0000242
name: error control parameter
namespace: KISAO
def: "Parameter controlling method accuracy." [:]
is_a: KISAO:0000201
disjoint_from: KISAO:0000252
disjoint_from: KISAO:0000243
disjoint_from: KISAO:0000244
created_by: AZ

[Term]
id: KISAO:0000243
name: method switching control parameter
namespace: KISAO
def: "Parameters describing threshold conditions for algorithms that switch between diffenet methods." [:]
is_a: KISAO:0000201
disjoint_from: KISAO:0000242
disjoint_from: KISAO:0000252
disjoint_from: KISAO:0000244
created_by: AZ

[Term]
id: KISAO:0000244
name: granularity control parameter
namespace: KISAO
def: "Parameter controlling granularity." [:]
is_a: KISAO:0000201
disjoint_from: KISAO:0000242
disjoint_from: KISAO:0000252
disjoint_from: KISAO:0000243
created_by: AZ

[Term]
id: KISAO:0000248
name: tau-leaping delta
namespace: KISAO
def: "Tau-leaping delta specifies how close two symmetric transition rates must be before we classify them as in partial-equilibrium. Only applies to the implicit tau routine." [:]
is_a: KISAO:0000252
disjoint_from: KISAO:0000249
disjoint_from: KISAO:0000204
disjoint_from: KISAO:0000203
disjoint_from: KISAO:0000205
disjoint_from: KISAO:0000260
disjoint_from: KISAO:0000258
disjoint_from: KISAO:0000257
relationship: KISAO:0000250 KISAO:0000045


[Term]
id: KISAO:0000249
name: critical firing threshold
namespace: KISAO
def: "The Nonnegative Poisson tau-leaping algorithm is based on the fact that negative populations typically arise from multiple firings of reactions that are only a few firings away from consuming all the molecules of one of their reactants. To focus on those reaction channels, the modified tau-leaping algorithm introduces a second control parameter nc, a positive integer that is usually set somewhere between 5 and 20. Any reaction channel with a positive propensity function that is currently within nc firings of exhausting one of its reactants is then classified as a critical reaction. The modified algorithm chooses tau in such a way that no more than one firing of all the critical reactions can occur during the leap." [:]
synonym: "nonnegative tau-leaping second control parameter" EXACT []
is_a: KISAO:0000252
disjoint_from: KISAO:0000204
disjoint_from: KISAO:0000203
disjoint_from: KISAO:0000205
disjoint_from: KISAO:0000260
disjoint_from: KISAO:0000258
disjoint_from: KISAO:0000248
disjoint_from: KISAO:0000257
relationship: KISAO:0000250 KISAO:0000084


[Term]
id: KISAO:0000252
name: partitioning control parameter
namespace: KISAO
is_a: KISAO:0000201
disjoint_from: KISAO:0000242
disjoint_from: KISAO:0000243
disjoint_from: KISAO:0000244
created_by: Parameter describing partitioning of the system.

[Term]
id: KISAO:0000253
name: coarse-graining factor
namespace: KISAO
def: "The time in each Monte-Carlo iteration is updated with the time increments tau=f/(a1+a2+...+aM). Here 1/(a1+a2+...+aM) is the averaged microscopic increment of the SSA and f is a coarse-graining factor, controlling the speed-up." [urn:miriam:pubmed:15638577 "Chatterjee A, Vlachos DG, Katsoulakis MA. Binomial distribution based -leap accelerated stochastic simulation. J Chem Phys. 2005;122(2):024112."]
is_a: KISAO:0000244
disjoint_from: KISAO:0000223
disjoint_from: KISAO:0000213
disjoint_from: KISAO:0000114
relationship: KISAO:0000250 KISAO:0000074


[Term]
id: KISAO:0000254
name: Brownian diffusion accuracy
namespace: KISAO
def: "Accuracy code, from 0 to 10. The accuracy statement sets which neighboring boxes are checked for potential bi-molecular reactions. Consider the reaction A + B -> C and suppose that A and B are within a binding radius of each other. This reaction will always be performed if A and B are in the same virtual box. If accuracy is set to at least 3, then it will also occur if A and B are in nearest-neighbor virtual boxes. If it is at least 7, then the reaction will happen if they are in nearest-neighbor boxes that are separated by periodic boundary conditions. And if it is 9 or 10, then all edge and corner boxes are checked for reactions, which means that no potential reactions are overlooked. Overall, increasing accuracy numbers lead to improved quantitative bimolecular reaction rates, along with substantially slower simulations. If qualitative simulations are wanted, then lower accuracy values are likely to be preferable [Smoldyn userguide]." [:]
is_a: KISAO:0000242
disjoint_from: KISAO:0000209
disjoint_from: KISAO:0000228
disjoint_from: KISAO:0000211
relationship: KISAO:0000250 KISAO:0000057


[Term]
id: KISAO:0000255
name: molecules per virtual box
namespace: KISAO
def: "Target molecules per virtual box. Sets the box sizes so that the average number of molecules per box, at simulation initiation, is close to the requested number. Good numbers tend to be between 3 and 6, although more or fewer may be appropriate, depending on how the number of molecules in the simulation is likely to change over time (the default box size is computed for an average of 4 molecules per box) [Smoldyn userguide]." [:]
is_a: KISAO:0000260
disjoint_from: KISAO:0000256

[Term]
id: KISAO:0000256
name: virtual box side length
namespace: KISAO
def: "The 'virtual box side length' statement requests the length of one side of a box, which should be in the same units that are used for the boundary statements [Smoldyn userguide]." [:]
is_a: KISAO:0000260
disjoint_from: KISAO:0000255

[Term]
id: KISAO:0000257
name: surface-bound epsilon
namespace: KISAO
def: "Molecules that are bound to a surface are given locations that are extremely close to that surface. However, this position does not need to be exactly at the surface, and in fact it usually cannot be exactly at the surface due to round-off error. The tolerance for how far a surface-bound molecule is allowed to be away from the surface can be set with the epsilon statement [Smoldyn userguide]." [:]
is_a: KISAO:0000252
disjoint_from: KISAO:0000249
disjoint_from: KISAO:0000204
disjoint_from: KISAO:0000203
disjoint_from: KISAO:0000205
disjoint_from: KISAO:0000260
disjoint_from: KISAO:0000258
disjoint_from: KISAO:0000248
relationship: KISAO:0000250 KISAO:0000057


[Term]
id: KISAO:0000258
name: neighbour distance
namespace: KISAO
def: "When a surface-bound molecule diffuses off of one surface panel, it can sometimes diffuse onto the neighbouring surface tile. It does so only if the neighbouring panel is declared to be a neighbour and also the neighbour is within a distance that is set with the neighbour distance statement. As a default, this distance is set to 3 times the longest surface-bound molecule rms step length [Smoldyn userguide]." [:]
is_a: KISAO:0000252
disjoint_from: KISAO:0000249
disjoint_from: KISAO:0000204
disjoint_from: KISAO:0000203
disjoint_from: KISAO:0000205
disjoint_from: KISAO:0000260
disjoint_from: KISAO:0000248
disjoint_from: KISAO:0000257
relationship: KISAO:0000250 KISAO:0000057


[Term]
id: KISAO:0000260
name: virtual box size
namespace: KISAO
def: "Target size of virtual boxes for 'Brownian diffusion Smoluchowski method'." [:]
is_a: KISAO:0000252
disjoint_from: KISAO:0000249
disjoint_from: KISAO:0000204
disjoint_from: KISAO:0000203
disjoint_from: KISAO:0000205
disjoint_from: KISAO:0000258
disjoint_from: KISAO:0000248
disjoint_from: KISAO:0000257
relationship: KISAO:0000250 KISAO:0000057


[Term]
id: KISAO:0000261
name: Euler method
namespace: KISAO
def: "The Euler method, named after Leonhard Euler, is a first-order numerical procedure for solving ordinary differential equations (ODEs) with a given initial value." [urn:miriam:isbn:052143064X "Press WH, Teukolsky SA, Vetterling WT, Flannery BP. Numerical Recipes in Fortran 77. Cambridge University Press (2001)."]
is_a: KISAO:0000000
disjoint_from: KISAO:0000056
disjoint_from: KISAO:0000264
disjoint_from: KISAO:0000087
disjoint_from: KISAO:0000033
disjoint_from: KISAO:0000032
disjoint_from: KISAO:0000241
disjoint_from: KISAO:0000094
disjoint_from: KISAO:0000086
disjoint_from: KISAO:0000017
disjoint_from: KISAO:0000019
disjoint_from: KISAO:0000064
disjoint_from: KISAO:0000231
relationship: KISAO:0000245 KISAO:0000108

relationship: KISAO:0000245 KISAO:0000103

relationship: KISAO:0000247 KISAO:0000102

relationship: KISAO:0000245 KISAO:0000106

created_by: AZ

[Term]
id: KISAO:0000262
name: deprecated class
def: "The root of the branch where all the deprecated terms are stored." [:]
is_obsolete: true
created_by: AZ

[Term]
id: KISAO:0000263
name: NFSim agent-based simulation method
namespace: KISAO
def: "To advance a simulation efficiently in time, we generalized a rule-based version of 'Gillespie's direct method' (SSA) [KISAO_0000029]. Our method is guaranteed to produce the same results as the exact SSA by cycling over three primary steps. First, NFsim calculates the probability or propensity for each rule to take effect given the current molecular states. Second, it samples the time to the next reaction event and selects the corresponding reaction rule. Finally, NFsim executes the selected reaction by applying the rule and updating the molecular agents accordingly." [urn:miriam:doi:10.1038/nmeth.1546 ""]
comment: Used in NFSim.
is_a: KISAO:0000017
creation_date: 2011-04-07T00:00:00Z
created_by: AZ

[Term]
id: KISAO:0000264
name: cellular automata update method
namespace: KISAO
def: "Cellular automata are mathematical idealizations of physical systems in which space and time are discrete, and physical quantities take on a finite set of discrete values. A cellular automaton consists of a regular uniform lattice (or ''array''), usually infinite in extent, with a discrete variable at each site (''cell''). A cellular automaton evolves in discrete time steps, with the value of the variable at one site being affected by the values of variables at sites in its ''neighborhood'' on the previous time step. The neighborhood of a site is typically taken to be the site itself and all immediately adjacent sites. The variables at each site are updated simultaneously (''synchronously''), based on the values of the variables in their neighborhood at the preceding time step, and according to a definite set of ''local rules''." [doi:10.1103/RevModPhys.55.601 "Wolfram, Stephen (1983) Statistical mechanics of cellular automata. Reviews of Modern Physics 55 (3): 601644."]
synonym: "tessellation automata" EXACT []
synonym: "iterative arrays" EXACT []
synonym: "cellular spaces" EXACT []
synonym: "cellular automata" EXACT []
synonym: "cellular structures" EXACT []
synonym: "homogeneous structures" EXACT []
synonym: "CA" EXACT []
synonym: "tessellation structures" EXACT []
is_a: KISAO:0000000
disjoint_from: KISAO:0000056
disjoint_from: KISAO:0000094
disjoint_from: KISAO:0000241
disjoint_from: KISAO:0000261
disjoint_from: KISAO:0000064
disjoint_from: KISAO:0000017
disjoint_from: KISAO:0000019
disjoint_from: KISAO:0000231
relationship: KISAO:0000245 KISAO:0000102

relationship: KISAO:0000245 KISAO:0000108

relationship: KISAO:0000245 KISAO:0000105

creation_date: 2011-04-07T00:00:00Z
created_by: AZ


! ----------------------  INSTANCES  -------------------------
